checkpoint.
- need to generalize instantiate to any [Pure-able] thing.

theories/RTac/Core.v
@@ -54,6 +54,7 @@ Section parameterized.
   Variable expr : Type.
 
   Context {RType_typ : RType typ}.
+  Context {RTypeOk_typ : RTypeOk}.
   Context {Expr_expr : Expr RType_typ expr}.
   Context {ExprOk_expr : ExprOk Expr_expr}.
   Context {Typ0_Prop : Typ0 _ Prop}.
@@ -70,8 +71,7 @@ Section parameterized.
 
   Inductive WellFormed_Goal (tus tvs : tenv typ) : Goal -> Prop :=
   | WFExs : forall ts s g,
-              FMapSubst.SUBST.WellFormed s ->
-              only_in_range (length tus) (length ts) s ->
+              WellFormed_pre_entry (length tus) (length ts) s ->
               WellFormed_Goal (tus ++ ts) tvs g ->
               WellFormed_Goal tus tvs (GExs ts s g)
   | WFAll : forall t g, WellFormed_Goal tus (tvs ++ t :: nil) g ->
@@ -96,19 +96,18 @@ Section parameterized.
   Global Instance Injective_WellFormed_Goal_GExs tus tvs l a g
   : Injective (WellFormed_Goal tus tvs (GExs l a g)) :=
     { result := WellFormed_Goal (tus ++ l) tvs g /\
-                WellFormed_amap a /\
-                only_in_range (length tus) (length l) a }.
+                WellFormed_pre_entry (length tus) (length l) a }.
   Proof.
     refine (fun pf =>
               match pf in WellFormed_Goal _ _ G
                     return match G return Prop with
-                             | GExs l a g => WellFormed_Goal (tus ++ l) tvs g /\
-                                             WellFormed_amap a /\
-                                             only_in_range (length tus) (length l) a
+                             | GExs l a g =>
+                               WellFormed_Goal (tus ++ l) tvs g /\
+                               WellFormed_pre_entry (length tus) (length l) a
                              | _ => True
                            end
               with
-                | WFExs _ _ _ a b c => conj c (conj a b)
+                | WFExs _ _ _ a b => conj b a
                 | _ => I
               end).
   Defined.
@@ -222,7 +221,10 @@ Section parameterized.
   End with_T.
   Definition nth_after T a b c := @nth_after' T b c a.
 
-  Definition hlist_get_cons_after_app {T : Type} {F : T -> Type} {t} {a b : list T}
+(*
+  (** NOTE: This definition is kind of in the way **)
+  Definition hlist_get_cons_after_app
+             {T : Type} {F : T -> Type} {t} {a b : list T}
              (h : hlist F (a ++ t :: b)) : F t :=
     (match nth_after a t b in _ = T return match T with
                                              | None => unit
@@ -232,7 +234,6 @@ Section parameterized.
        | eq_refl => hlist_nth h (length a)
      end).
 
-(*
   Fixpoint goal_substD (tus tvs : list typ)
            (ts : list typ) (es : list (option expr))
   : option (exprT (tus ++ ts) tvs Prop) :=
