theories/RTac/Then.v
@@ -8,10 +8,11 @@ Set Implicit Arguments.
 Set Strict Implicit.
 
 Section parameterized.
-  Variable typ : Type.
-  Variable expr : Type.
+  Context {typ : Type}.
+  Context {expr : Type}.
 
   Context {RType_typ : RType typ}.
+  Context {RTypeOk_typ : RTypeOk}.
   Context {Expr_expr : Expr RType_typ expr}.
   Context {Typ0_Prop : Typ0 _ Prop}.
 
