theories/RTac/Try.v
@@ -11,6 +11,7 @@ Section parameterized.
   Context {expr : Type}.
   Context {subst : Type}.
   Context {RType_typ : RType typ}.
+  Context {RTypeOk_typ : RTypeOk}.
   Context {Expr_expr : Expr RType_typ expr}.
   Context {Typ0_Prop : Typ0 _ Prop}.
 
